ArchAcc_AI checks with new subgoal command

lib/Eisbach_Methods.thy
@@ -1,22 +1,130 @@
 (* Some useful boilerplate methods for Eisbach *)
 
 theory Eisbach_Methods
-imports "~~/src/HOL/Eisbach/Eisbach_Tools"
+imports "~~/src/HOL/Eisbach/Eisbach_Tools" 
+        "wp/NonDetMonadVCG" 
+        "subgoal_focus/Subgoal_Focus"
+        "subgoal_focus/Subgoal_Methods"
 begin
 
 ML \<open>fun DROP_CASES f xq = (Seq.map snd o f) xq\<close>
 
 (* Focus without matching. No focus elements are available directly. *)
 method_setup focus = \<open>
-  Method_Closure.parse_method >> (fn m => fn ctxt => fn facts => 
+  Scan.lift (Args.mode "concl") -- Method_Closure.parse_method >> (fn (b,m) => fn ctxt => fn facts => 
   let
     val m' = Method_Closure.method_evaluate m;
+    val focus = if b then Subgoal.FOCUS else Subgoal.FOCUS_PARAMS; 
   in
-   Subgoal.FOCUS (fn {context,...} => DROP_CASES (m' context facts)) ctxt 1
+   focus (fn {context,...} => DROP_CASES (m' context facts)) ctxt 1
    |> EMPTY_CASES
    end)
 \<close>
 
+method_setup all =
+ \<open>Method_Closure.parse_method >> (fn m => fn ctxt => fn facts =>
+   let
+     fun tac i st' =
+       Goal.restrict i 1 st'
+       |> Method_Closure.method_evaluate m ctxt facts
+       |> Seq.map (Goal.unrestrict i o snd)
+
+   in EMPTY_CASES (ALLGOALS tac) end)
+\<close>
+
 method print_concl = (match conclusion in P for P \<Rightarrow> \<open>print_term P\<close>)
+
+method_setup print_goal = \<open>Scan.succeed (fn ctxt => fn facts => 
+  (fn st => (Output.writeln (Display.string_of_thm ctxt st); Seq.single ([],st))))\<close>
+
+
+definition "packed_valid P f si r s \<equiv> P si \<and> (r, s) \<in> fst (f si)"
+
+lemma packed_validE:"(\<And>si r s. packed_valid P f si r s \<Longrightarrow> Q r s) \<Longrightarrow> \<lbrace>P\<rbrace> f \<lbrace>Q\<rbrace>"
+  by (clarsimp simp: valid_def packed_valid_def)
+
+lemma packed_validI: "\<lbrace>P\<rbrace> f \<lbrace>Q\<rbrace> \<Longrightarrow> \<forall>si r s. packed_valid P f si r s \<longrightarrow> Q r s"
+  apply (clarsimp simp: valid_def packed_valid_def)
+  by auto
+
+definition "packed_validR P f si r s \<equiv> P si \<and> (Inr r, s) \<in> fst (f si)"
+
+
+lemma packed_validRE:"(\<And>si r s. packed_validR P f si r s \<Longrightarrow> Q r s) \<Longrightarrow> \<lbrace>P\<rbrace> f \<lbrace>Q\<rbrace>,-"
+  apply (clarsimp simp: validE_R_def validE_def valid_def packed_validR_def)
+  by (metis sum.case sumE)
+
+lemma packed_validRI: "\<lbrace>P\<rbrace> f \<lbrace>Q\<rbrace>,- \<Longrightarrow> \<forall>si r s. packed_validR P f si r s \<longrightarrow> Q r s"
+  apply (clarsimp simp: valid_def validE_R_def validE_def packed_validR_def)
+  by fastforce
+
+lemma trivial_imp: "\<forall>r s. Q r s \<longrightarrow> Q r s" by simp
+
+lemma uncurry2: "\<forall>r s. Q r s \<and> Q' r s \<longrightarrow> Q'' r s \<Longrightarrow> \<forall>r s. Q r s \<longrightarrow> Q' r s \<longrightarrow> Q'' r s"
+  by simp
+
+
+named_theorems hoare_post_imps
+
+lemmas [hoare_post_imps] = hoare_post_imp_R hoare_post_imp[rotated]
+
+method post_asm_raw methods m = 
+  (drule hoare_post_imps,
+   atomize (full),
+   focus (concl) 
+     \<open>intro impI allI, 
+      m, 
+      atomize (full),
+      ((rule uncurry2)+)?\<close>,
+   rule trivial_imp)
+
+method post_asm methods m = 
+  (post_asm_raw \<open>(simp only: bipred_conj_def pred_conj_def)?,(elim conjE)?,m\<close>)
+
+
+named_theorems packed_validEs
+
+lemmas [packed_validEs] = packed_validE packed_validRE
+
+named_theorems packed_validIs
+
+lemmas [packed_validIs] = packed_validI packed_validRI
+
+method post_raw methods m = 
+  (focus 
+    \<open>rule packed_validEs,
+     focus (concl) \<open>m,fold_subgoals\<close>, 
+     atomize (full),
+     rule packed_validI\<close>)
+
+method post methods m = 
+  (post_raw 
+     \<open>intro impI conjI allI,
+      distinct_subgoals,
+      all \<open>m\<close>,
+      fold_subgoals\<close>)
+
+context
+begin
+
+private definition "protect_concl x \<equiv> \<not> x"
+private definition "protect_false \<equiv> False"
+
+private lemma protect_start: "(protect_concl P \<Longrightarrow> protect_false) \<Longrightarrow> P" 
+  by (simp add: protect_concl_def protect_false_def) (rule ccontr)
+
+private lemma protect_end: "protect_concl P \<Longrightarrow> P \<Longrightarrow> protect_false" 
+  by (simp add: protect_concl_def protect_false_def)
+
+method only_asm methods m = 
+  (match premises in H[thin]:_ (multi) \<Rightarrow> 
+    \<open>rule protect_start, 
+     match premises in H'[thin]:"protect_concl _" \<Rightarrow> 
+       \<open>insert H,m;rule protect_end[OF H']\<close>\<close>)
+
+method only_concl methods m = (match premises in _ (multi) \<Rightarrow> \<open>m\<close>)
+
+end
+
 
 end
