lib/NICTATools.thy
@@ -14,9 +14,10 @@ imports
 (* Apply_Trace_Cmd *) 
   Solves_Tac
   "subgoal_focus/Subgoal_Focus"
-  "subgoal_focus/Noting"
   "subgoal_focus/Subgoal_Methods"
+  "subgoal_focus/Rule_By_Method"
   Eisbach_Methods
+  "~~/src/HOL/Eisbach/Eisbach_Tools"
 begin
 
 section "Detect unused meta-forall"
